vale/code/arch/x64/X64.Vale.Lemmas.fst
@@ -3,31 +3,30 @@ open X64.Machine_s
 open X64.Vale.State
 open X64.Vale.StateLemmas
 module BS = X64.Bytes_Semantics_s
-module TS = X64.Taint_Semantics_s
 module ME = X64.Memory
 
 friend X64.Vale.StateLemmas
 
-#reset-options "--initial_fuel 2 --max_fuel 2 --z3rlimit 20"
+#reset-options "--initial_fuel 2 --max_fuel 2 --z3rlimit 30"
 
 val eval_code_eq_all (c:code) (f:fuel) : Lemma
-  (ensures (forall (s1 s2:BS.machine_state).{:pattern (TS.taint_eval_code c f s1); (TS.taint_eval_code c f s2)}
+  (ensures (forall (s1 s2:BS.machine_state).{:pattern (BS.machine_eval_code c f s1); (BS.machine_eval_code c f s2)}
     state_eq_S s1 s2 ==>
-    state_eq_opt (TS.taint_eval_code c f s1) (TS.taint_eval_code c f s2)
+    state_eq_opt (BS.machine_eval_code c f s1) (BS.machine_eval_code c f s2)
   ))
   (decreases %[f; c; 1])
 
 val eval_codes_eq_all (cs:codes) (f:fuel) : Lemma
-  (ensures (forall (s1 s2:BS.machine_state).{:pattern (TS.taint_eval_codes cs f s1); (TS.taint_eval_codes cs f s2)}
+  (ensures (forall (s1 s2:BS.machine_state).{:pattern (BS.machine_eval_codes cs f s1); (BS.machine_eval_codes cs f s2)}
     state_eq_S s1 s2 ==>
-    state_eq_opt (TS.taint_eval_codes cs f s1) (TS.taint_eval_codes cs f s2)
+    state_eq_opt (BS.machine_eval_codes cs f s1) (BS.machine_eval_codes cs f s2)
   ))
   (decreases %[f; cs])
 
 val eval_while_eq_all (c:code) (f:fuel) : Lemma
-  (ensures (forall (s1 s2:BS.machine_state).{:pattern (TS.taint_eval_while c f s1); (TS.taint_eval_while c f s2)}
+  (ensures (forall (s1 s2:BS.machine_state).{:pattern (BS.machine_eval_while c f s1); (BS.machine_eval_while c f s2)}
     While? c /\ state_eq_S s1 s2 ==>
-    state_eq_opt (TS.taint_eval_while c f s1) (TS.taint_eval_while c f s2)
+    state_eq_opt (BS.machine_eval_while c f s1) (BS.machine_eval_while c f s2)
   ))
   (decreases %[f; c; 0])
 
@@ -49,27 +48,27 @@ and eval_while_eq_all c f =
 
 let eval_code_eq (c:code) (f:fuel) (s1 s2:BS.machine_state) : Lemma
   (requires state_eq_S s1 s2)
-  (ensures state_eq_opt (TS.taint_eval_code c f s1) (TS.taint_eval_code c f s2))
-  [SMTPat (TS.taint_eval_code c f s1); SMTPat (TS.taint_eval_code c f s2)]
+  (ensures state_eq_opt (BS.machine_eval_code c f s1) (BS.machine_eval_code c f s2))
+  [SMTPat (BS.machine_eval_code c f s1); SMTPat (BS.machine_eval_code c f s2)]
   =
   eval_code_eq_all c f
 
 let eval_codes_eq (cs:codes) (f:fuel) (s1 s2:BS.machine_state) : Lemma
   (requires state_eq_S s1 s2)
-  (ensures state_eq_opt (TS.taint_eval_codes cs f s1) (TS.taint_eval_codes cs f s2))
-  [SMTPat (TS.taint_eval_codes cs f s1); SMTPat (TS.taint_eval_codes cs f s2)]
+  (ensures state_eq_opt (BS.machine_eval_codes cs f s1) (BS.machine_eval_codes cs f s2))
+  [SMTPat (BS.machine_eval_codes cs f s1); SMTPat (BS.machine_eval_codes cs f s2)]
   =
   eval_codes_eq_all cs f
 
 let eval_while_eq (c:code) (f:fuel) (s1 s2:BS.machine_state) : Lemma
   (requires While? c /\ state_eq_S s1 s2)
-  (ensures state_eq_opt (TS.taint_eval_while c f s1) (TS.taint_eval_while c f s2))
-  [SMTPat (TS.taint_eval_while c f s1); SMTPat (TS.taint_eval_while c f s2)]
+  (ensures state_eq_opt (BS.machine_eval_while c f s1) (BS.machine_eval_while c f s2))
+  [SMTPat (BS.machine_eval_while c f s1); SMTPat (BS.machine_eval_while c f s2)]
   =
   eval_while_eq_all c f
 
 let eval_code_ts (c:code) (s0:BS.machine_state) (f0:fuel) (s1:BS.machine_state) : Type0 =
-  state_eq_opt (TS.taint_eval_code c f0 s0) (Some s1)
+  state_eq_opt (BS.machine_eval_code c f0 s0) (Some s1)
 
 val increase_fuel (c:code) (s0:BS.machine_state) (f0:fuel) (sN:BS.machine_state) (fN:fuel) : Lemma
   (requires eval_code_ts c s0 f0 sN /\ f0 <= fN)
@@ -86,15 +85,15 @@ let rec increase_fuel c s0 f0 sN fN =
   | Ins ins -> ()
   | Block l -> increase_fuels l s0 f0 sN fN
   | IfElse b t f ->
-      let (_, b0) = TS.taint_eval_ocmp s0 b in
+      let (_, b0) = BS.machine_eval_ocmp s0 b in
       if b0 then increase_fuel t s0 f0 sN fN else increase_fuel f s0 f0 sN fN
   | While b c ->
-      let (s1, b0) = TS.taint_eval_ocmp s0 b in
+      let (s1, b0) = BS.machine_eval_ocmp s0 b in
       if not b0 then ()
       else
       (
         let s1 = {s1 with BS.ms_trace = BranchPredicate(true)::s1.BS.ms_trace} in
-        match TS.taint_eval_code c (f0 - 1) s1 with
+        match BS.machine_eval_code c (f0 - 1) s1 with
         | None -> ()
         | Some s2 ->
             increase_fuel c s1 (f0 - 1) s2 (fN - 1);
@@ -107,7 +106,7 @@ and increase_fuels c s0 f0 sN fN =
   | [] -> ()
   | h::t ->
     (
-      let Some s1 = TS.taint_eval_code h f0 s0 in
+      let Some s1 = BS.machine_eval_code h f0 s0 in
       increase_fuel h s0 f0 s1 fN;
       increase_fuels t s1 f0 sN fN
     )
@@ -147,9 +146,9 @@ let lemma_ifElseFalse_total (ifb:ocmp) (ct:code) (cf:code) (s0:state) (f0:fuel) 
   ()
 
 let eval_while_inv_temp (c:code) (s0:state) (fW:fuel) (sW:state) : Type0 =
-  forall (f:nat).{:pattern TS.taint_eval_code c f (state_to_S sW)}
-    Some? (TS.taint_eval_code c f (state_to_S sW)) ==>
-    state_eq_opt (TS.taint_eval_code c (f + fW) (state_to_S s0)) (TS.taint_eval_code c f (state_to_S sW))
+  forall (f:nat).{:pattern BS.machine_eval_code c f (state_to_S sW)}
+    Some? (BS.machine_eval_code c f (state_to_S sW)) ==>
+    state_eq_opt (BS.machine_eval_code c (f + fW) (state_to_S s0)) (BS.machine_eval_code c f (state_to_S sW))
 
 let eval_while_inv (c:code) (s0:state) (fW:fuel) (sW:state) : Type0 =
   eval_while_inv_temp c s0 fW sW
@@ -162,7 +161,7 @@ let lemma_whileTrue_total (b:ocmp) (c:code) (s0:state) (sW:state) (fW:fuel) =
 
 let lemma_whileFalse_total (b:ocmp) (c:code) (s0:state) (sW:state) (fW:fuel) =
   let f1 = fW + 1 in
-  assert (state_eq_opt (TS.taint_eval_code (While b c) f1 (state_to_S s0)) (TS.taint_eval_code (While b c) 1 (state_to_S sW)));
+  assert (state_eq_opt (BS.machine_eval_code (While b c) f1 (state_to_S s0)) (BS.machine_eval_code (While b c) 1 (state_to_S sW)));
   assert (eval_code (While b c) s0 f1 sW);
   (sW, f1)
 
@@ -170,26 +169,26 @@ let lemma_whileFalse_total (b:ocmp) (c:code) (s0:state) (sW:state) (fW:fuel) =
 let lemma_whileMerge_total (c:code) (s0:state) (f0:fuel) (sM:state) (fM:fuel) (sN:state) =
   let fN:nat = f0 + fM + 1 in
   let lForall () : Lemma
-    (forall (f:nat).{:pattern (TS.taint_eval_code c f (state_to_S sN))}
-      Some? (TS.taint_eval_code c f (state_to_S sN)) ==>
-      state_eq_opt (TS.taint_eval_code c (f + fN) (state_to_S s0)) (TS.taint_eval_code c f (state_to_S sN))
+    (forall (f:nat).{:pattern (BS.machine_eval_code c f (state_to_S sN))}
+      Some? (BS.machine_eval_code c f (state_to_S sN)) ==>
+      state_eq_opt (BS.machine_eval_code c (f + fN) (state_to_S s0)) (BS.machine_eval_code c f (state_to_S sN))
     ) =
     let fForall (f:nat) : Lemma
-      (requires Some? (TS.taint_eval_code c f (state_to_S sN)))
-      (ensures state_eq_opt (TS.taint_eval_code c (f + fN) (state_to_S s0)) (TS.taint_eval_code c f (state_to_S sN))) =
-      let Some sZ = TS.taint_eval_code c f (state_to_S sN) in
+      (requires Some? (BS.machine_eval_code c f (state_to_S sN)))
+      (ensures state_eq_opt (BS.machine_eval_code c (f + fN) (state_to_S s0)) (BS.machine_eval_code c f (state_to_S sN))) =
+      let Some sZ = BS.machine_eval_code c f (state_to_S sN) in
       let fZ = if f > fM then f else fM in
       increase_fuel (While?.whileBody c) (state_to_S sM) fM (state_to_S sN) fZ;
       
       increase_fuel c (state_to_S sN) f sZ fZ;
       
-      assert (state_eq_opt (TS.taint_eval_code c (fZ + 1) (state_to_S sM)) (Some sZ)); // via eval_code for While
-      assert (state_eq_opt (TS.taint_eval_code c (fZ + 1) (state_to_S sM)) (TS.taint_eval_code c (fZ + 1 + f0) (state_to_S s0))); // via eval_while_inv, choosing f = fZ + 1
+      assert (state_eq_opt (BS.machine_eval_code c (fZ + 1) (state_to_S sM)) (Some sZ)); // via eval_code for While
+      assert (state_eq_opt (BS.machine_eval_code c (fZ + 1) (state_to_S sM)) (BS.machine_eval_code c (fZ + 1 + f0) (state_to_S s0))); // via eval_while_inv, choosing f = fZ + 1
 
-      // Two assertions above prove (TS.taint_eval_code c (fZ + 1 + f0) (state_to_S s0)) equals (Some sZ)
+      // Two assertions above prove (BS.machine_eval_code c (fZ + 1 + f0) (state_to_S s0)) equals (Some sZ)
       // increase_fuel c s0 (fZ + 1 + f0) (state_of_S s0 sZ) (f + fN);
       increase_fuel c (state_to_S s0) (fZ + 1 + f0) sZ (f + fN);
-      assert (state_eq_opt (TS.taint_eval_code c (f + fN) (state_to_S s0)) (Some sZ));
+      assert (state_eq_opt (BS.machine_eval_code c (f + fN) (state_to_S s0)) (Some sZ));
       ()
       in
     Classical.ghost_lemma fForall
