vale/code/arch/x64/X64.Bytes_Semantics.fsti
@@ -1,6 +1,5 @@
 module X64.Bytes_Semantics
 
-module TS = X64.Taint_Semantics_s
 open X64.Bytes_Semantics_s
 open X64.Machine_s
 open Words_s
@@ -63,9 +62,9 @@ val same_mem_get_heap_val128 (ptr:int) (mem1 mem2:heap) : Lemma
   (ensures forall i. i >= ptr /\ i < ptr + 16 ==> mem1.[i] == mem2.[i])
 
 val eval_ins_domains (ins:ins) (s0:machine_state) : Lemma
-  (let s1 = TS.taint_eval_ins ins s0 in
-  Set.equal (Map.domain s0.ms_mem) (Map.domain s1.ms_mem))
+  ( let s1 = machine_eval_ins ins s0 in
+    Set.equal (Map.domain s0.ms_mem) (Map.domain s1.ms_mem))
 
 val eval_ins_same_unspecified (ins:ins) (s0:machine_state) : Lemma
-  (let Some s1 = TS.taint_eval_code (Ins ins) 0 s0 in
-   forall x. not (Map.contains s1.ms_mem x) ==> s1.ms_mem.[x] == s0.ms_mem.[x])
+  ( let Some s1 = machine_eval_code (Ins ins) 0 s0 in
+    forall x. not (Map.contains s1.ms_mem x) ==> s1.ms_mem.[x] == s0.ms_mem.[x])
