vale/code/arch/x64/interop/Vale.AsLowStar.ValeSig.fst
@@ -5,7 +5,6 @@ module BS = X64.Bytes_Semantics_s
 module BV = LowStar.BufferView
 module HS = FStar.HyperStack
 module ME = X64.Memory
-module TS = X64.Taint_Semantics_s
 module MS = X64.Machine_s
 module IA = Interop.Assumptions
 module V = X64.Vale.Decls
